ironfleet/src/Dafny/Distributed/Services/Lock/Compatible.i.dfy
@@ -1,0 +1,170 @@
+include "../../Concur/QuantizedSystem.s.dfy"
+   
+module Compatible_i {
+    import opened QuantizedSystem_s
+
+    /////////////////////////////////////////
+    // CanonicalAction definition
+    /////////////////////////////////////////
+
+    predicate IoCanMoveLeft(io:LIoOp)
+    {
+        io.LIoOpSend?
+    }
+
+    predicate IoCanMoveRight(io:LIoOp)
+    {
+        io.LIoOpReceive?
+    }
+
+    predicate IoCantMove(io:LIoOp)
+    {
+        !io.LIoOpSend? && !io.LIoOpReceive?
+    }
+
+    // Use lemma_CanonicalActionIsWellPositioned to demonstrate that
+    // CanonicalAction works, i.e., if the I/O sequence is compatible with
+    // reduction then every I/O before the canonical action is a
+    // right-mover and every I/O after the canonical action is a
+    // left-mover.
+
+    function CanonicalAction(ios:IoTrace) : int
+        requires |ios| > 0;
+        ensures  0 <= CanonicalAction(ios) < |ios|;
+    {
+        if exists i :: 0 <= i < |ios| && IoCantMove(ios[i]) then
+            // Choose the sole non-mover, if it exists
+            var i :| 0 <= i < |ios| && IoCantMove(ios[i]);
+            i
+        else if exists i :: 0 <= i < |ios| && IoCanMoveLeft(ios[i]) && (i == 0 || IoCanMoveRight(ios[i-1])) then
+            // Else choose the left-most left-mover, if there are any
+            var i :| 0 <= i < |ios| && IoCanMoveLeft(ios[i]) && (i == 0 || IoCanMoveRight(ios[i-1]));
+            i
+        else 
+            // Else choose the right-most right mover (at this point, we know every I/O is a right-mover)
+            |ios| - 1
+    }
+
+    ///////////////////////////////////////////////////////////////
+    // Choosing the minimum of a set of non-negative numbers
+    ///////////////////////////////////////////////////////////////
+
+    lemma lemma_MinimumOfNatSetHelper(s:set<int>)
+        requires  |s| > 0;
+        requires  forall i :: i in s ==> i >= 0;
+        ensures   exists j :: j in s && forall i :: i in s ==> i >= j;
+        decreases |s|;
+    {
+        var j :| j in s;
+        if k :| k in s && k < j {
+            var s' := s - {j};
+            lemma_MinimumOfNatSetHelper(s');
+            var j' :| j' in s' && forall i :: i in s' ==> i >= j';
+            forall i | i in s
+                ensures i >= j';
+            {
+                if i == j {
+                    assert k in s';
+                }
+                else {
+                    assert i in s';
+                }
+            }
+        }
+    }
+
+    function MinimumOfNatSet(s:set<int>) : int
+        requires |s| > 0;
+        requires forall i :: i in s ==> i >= 0;
+        ensures  MinimumOfNatSet(s) in s;
+        ensures  forall i :: i in s ==> MinimumOfNatSet(s) <= i;
+    {
+        lemma_MinimumOfNatSetHelper(s);
+        var j :| j in s && forall i :: i in s ==> i >= j;
+        j
+    }
+
+    ///////////////////////////////////////////////////////////////
+    // Helpers to show CanonicalAction works
+    ///////////////////////////////////////////////////////////////
+    
+    lemma lemma_IfCanonicalActionOptionThreeThenAllRightMovers(ios:IoTrace)
+        requires |ios| > 0;
+        requires LIoOpSeqCompatibleWithReduction(ios);
+        requires forall i :: 0 <= i < |ios| ==> !IoCantMove(ios[i]);
+        requires forall i :: 0 <= i < |ios| ==> !(IoCanMoveLeft(ios[i]) && (i == 0 || IoCanMoveRight(ios[i-1])));
+        ensures  forall i :: 0 <= i < |ios| ==> IoCanMoveRight(ios[i]);
+    {
+        if j :| 0 <= j < |ios| && !IoCanMoveRight(ios[j]) {
+            var left_movers := set k | 0 <= k < |ios| && !IoCanMoveRight(ios[k]);
+            assert j in left_movers;
+            assert |left_movers| > 0;
+            var min_left_mover := MinimumOfNatSet(left_movers);
+            assert min_left_mover - 1 !in left_movers;
+            assert IoCanMoveLeft(ios[min_left_mover]) && (min_left_mover == 0 || IoCanMoveRight(ios[min_left_mover - 1]));
+            assert false;
+        }
+    }
+
+    lemma lemma_CanonicalActionIsWellPositionedHelperLeft(ios:IoTrace, i:int)
+        requires |ios| > 0;
+        requires LIoOpSeqCompatibleWithReduction(ios);
+        requires 0 <= i < CanonicalAction(ios);
+        ensures  IoCanMoveRight(ios[i]);
+        decreases CanonicalAction(ios) - i;
+    {
+        var a := CanonicalAction(ios);
+        if i == a - 1 {
+            assert LIoOpOrderingOKForAction(ios[i], ios[i+1]);
+            if !IoCanMoveRight(ios[i]) {
+                lemma_IfCanonicalActionOptionThreeThenAllRightMovers(ios);
+            }
+        }
+        else {
+            lemma_CanonicalActionIsWellPositionedHelperLeft(ios, i+1);
+            assert LIoOpOrderingOKForAction(ios[i], ios[i+1]);
+        }
+    }
+
+    lemma lemma_CanonicalActionIsWellPositionedHelperRight(ios:IoTrace, i:int)
+        requires |ios| > 0;
+        requires LIoOpSeqCompatibleWithReduction(ios);
+        requires CanonicalAction(ios) < i < |ios|;
+        ensures  IoCanMoveLeft(ios[i]);
+        decreases i;
+    {
+        var a := CanonicalAction(ios);
+        if i == a + 1 {
+            assert LIoOpOrderingOKForAction(ios[a], ios[a+1]);
+        }
+        else {
+            lemma_CanonicalActionIsWellPositionedHelperRight(ios, i-1);
+            assert LIoOpOrderingOKForAction(ios[i-1], ios[(i-1)+1]);
+        }
+    }
+
+    ///////////////////////////////////////////////////////////////
+    // Lemma showing CanonicalAction works
+    ///////////////////////////////////////////////////////////////
+
+    lemma lemma_CanonicalActionIsWellPositioned(ios:IoTrace)
+        requires |ios| > 0;
+        requires LIoOpSeqCompatibleWithReduction(ios);
+        ensures  forall i :: 0 <= i < CanonicalAction(ios) ==> IoCanMoveRight(ios[i]);
+        ensures  forall i :: CanonicalAction(ios) < i < |ios| ==> IoCanMoveLeft(ios[i]);
+    {
+        var a := CanonicalAction(ios);
+        forall i | 0 <= i < a
+            ensures IoCanMoveRight(ios[i]);
+        {
+            lemma_CanonicalActionIsWellPositionedHelperLeft(ios, i);
+        }
+
+        forall i | a < i < |ios|
+            ensures IoCanMoveLeft(ios[i]);
+        {
+            lemma_CanonicalActionIsWellPositionedHelperRight(ios, i);
+        }
+    }
+
+}
